Lean4Lean/Verify/Typing/Expr.lean
@@ -60,7 +60,7 @@ def VLCtx.WF : VLCtx → Prop
     VLCtx.WF Δ ∧ (∀ fv deps, ofv = some (fv, deps) → fv ∉ Δ.fvars ∧ deps ⊆ Δ.fvars) ∧
     VLocalDecl.WF env U Δ.toCtx d
 
-def VLCtx.WF.fvwf : ∀ {Δ}, VLCtx.WF env U Δ → Δ.FVWF
+theorem VLCtx.WF.fvwf : ∀ {Δ}, VLCtx.WF env U Δ → Δ.FVWF
   | [], h => h
   | _ :: _, ⟨h1, h2, _⟩ => ⟨h1.fvwf, h2⟩
 
